%\documentclass[border=10pt,tikz,letter]{standalone}
\documentclass[10pt,british,letter]{ltxdoc}
\usepackage{prooftrees,turnstile}
\newcommand*{\lif}{\ensuremath{\mathbin{\rightarrow}}}

\newcommand\vver[1]{\textcolor{red}{\textit{#1 }}}

\begin{document}

\begin{prooftree}
{
  to prove={(A \vee B) \lif (A \wedge B), A \vee B \sststile{}{} A \wedge B}
}
  [\vver{v} (A \vee B) \lif (A \wedge B), just=Premisa, name=p1
    [\vver{v} A \vee B, just=Premisa
        [\vver{f} A \wedge B, just=Conclusión
          [\vver{f} A \vee B, just={VI:p1}, close]
          [\vver{v} A \wedge B, close]
        ]
      ]
    ]
  ]
\end{prooftree}

\begin{prooftree}
  {
    to prove={(C \vee D) \lif (C \wedge D), C \wedge D \sststile{}{} C \vee D}
  }
  [\vver{v} (C \vee D) \lif (C \wedge D), just=Premisa, name=p1
    [\vver{v} C \wedge D, just=Premisa, name=p2
      [\vver{f} C \vee D, just=Conclusión, name=conc
        [\vver{f} C \vee D, just=VI:p1, name=via
          [\vver{f} C, just=FD:via
            [\vver{f} D, just=FD:via
              [\vver{v} C, just=VC:p2
                [\vver{v} D, close, just=VC:p2]
              ]
            ]
          ]
        ]
        [\vver{v} C \wedge D, just=VI:p1, name=vic
          [\vver{v} C, just=VC:vic
            [\vver{v} D, just=VC:vic
              [\vver{f} C, just=FD:conc
                [\vver{f} D, close, just=FD:conc]
              ]
            ]
          ]
        ]
      ]
    ]
  ]
\end{prooftree}

\begin{prooftree}
  {
    to prove={E \lif F, F \lif E \sststile{}{} E \vee F}
  }
  [\vver{v} E \lif F, name=prem1
    [\vver{v} F \lif E, name=prem2
      [\vver{f} E \vee F, name=conc
        [\vver{f} E, just=FD:conc, name=fdconc
          [\vver{f} F, just=FD:conc
            [\vver{f} F, just=VI:prem2, name=viprem2
              [\vver{f} E, just=VI:prem1]
              [\vver{v} F, close={:viprem2,!c}, just=VI:prem1]
            ]
            [\vver{v} E, close={:fdconc,!c}, just=VI:prem2]
          ]
        ]
      ]
    ]
  ]
\end{prooftree}

% \item
\begin{prooftree}
  {
    to prove={(G \vee H) \lif (G \wedge H), \lnot (G \wedge H) \sststile{}{} \lnot (G \vee H)}
  }
  [\vver{v} (G \vee H) \lif (G \wedge H), name=prem1
    [\vver{v} \lnot (G \wedge H), name=prem2
      [\vver{f} \lnot (G \vee H), name=conc
        [\vver{f} (G \wedge H), just=NG:prem2, name=negprem2
          [\vver{v} (G \vee H), just=NG:conc, name=negcon
            [\vver{f} (G \vee H), just=VI:prem1, close={:negcon,!c}]
            [\vver{v} (G \wedge H), just=VI:prem1, close={:negprem2,!c}]
          ]
        ]
      ]
    ]
  ]
\end{prooftree}

% \item
\begin{prooftree}
  {
    to prove={(I \vee J) \lif (I \wedge J), \lnot(I \vee J) \sststile{}{} \lnot (I \wedge J)}
  }
  [\vver{v} (I \vee J) \lif (I \wedge J), name=prem1
    [\vver{v} \lnot(I \vee J), name=prem2
      [\vver{f} \lnot (I \wedge J), name=conc
        [\vver{f} I \vee J, name=ngprem1, just=NG:prem2
          [\vver{v} I \wedge J, name=ngconc, just=NG:conc
            [\vver{f} I, just=FD:ngprem1, name=faldisant
              [\vver{f} J, just=FD:ngprem1, name=faldiscon
                [\vver{v} I, just=VC:ngconc, close={:faldisant,!c}
                  [\vver{v} J, just=VC:ngconc, close={:faldiscon,!c}
                    % [\vver{f} I \vee J, name=viprem1ant, just=VI:prem1
                    %   [\vver{f} I, just=FD:viprem1ant
                    %     [\vver{f} J, just=FD:viprem1ant, close={,!c}]
                    %   ]
                    % ]
                    % [\vver{v} I \wedge J, name=viprem1con, just=VI:prem1
                    %   [\vver{v} I, just=VC:viprem1con
                    %     [\vver{v} J, just=VC:viprem1con, close={,!c}]
                    %   ]
                    % ]
                  ]
                ]
              ]
            ]
          ]
        ]
      ]
    ]
  ]
\end{prooftree}

% \item
\begin{prooftree}
  {
    to prove={K \vee L, K \sststile{}{} \lnot L }
  }
  [\vver{v} K \vee L, name=prem1, just=Premisa
    [\vver{v} K, name=prem2, just=Premisa
      [\vver{f} \lnot L, name=conc, just=Conclusión
        [\vver{v} K, just=VD:prem1, name=vdPrem1]
        [\vver{v} L, just=VD:prem1, close={:vdPrem1,!c}]
      ]
    ]
  ]
\end{prooftree}

% \item
\begin{prooftree}
  {
    to prove={M \vee (N \wedge \lnot N), M \sststile{}{} \lnot(N \wedge \lnot N)}
  }
  [\vver{v} M \vee (N \wedge \lnot N), name=prem1, just=Premisa
    [\vver{v} M, name=prem2,just=Premisa
      [\vver{f} \lnot (N \wedge \lnot N), name=conc,just=Conclusión
        [\vver{v} N \wedge \lnot N, just=DN:conc, name=dnConc
          [\vver{v} N, just=VC:dnConc
            [\vver{v} \lnot N, just=VC:dnConc]
          ]
        ]
      ]
    ]
  ]
\end{prooftree}

% \item
\begin{prooftree}
  {
    to prove={(O \vee P) \lif Q, Q \lif (O \wedge P) \sststile{}{} (O \vee P) \lif (O \wedge P)}
  }
  [\vver{v} (O \vee P) \lif Q, name=prem1,just=Premisa
    [\vver{v} Q \lif (O \wedge P), name=prem2,just=Premisa
      [\vver{f} (O \vee P) \lif (O \wedge P), name=conc,just=Conclusión
        [\vver{v} O \vee P, just=FI:conc, name=fiConcAnt
          [\vver{f} O \wedge P, just=FI:conc, name=fiConcCon
            [\vver{f} O \vee P, close={:fiConcAnt,!c}, just=VI:prem1]
            [\vver{v} Q, just=VI:prem1, name=viPrem1
              [\vver{f} Q, close={:viPrem1,!c}]
              [\vver{v} O \wedge P, close={:fiConcCon,!c}]
            ]
          ]
        ]
      ]
    ]
  ]
\end{prooftree}

% \item
\begin{prooftree}
  {
    to prove={(R \vee S) \lif T, T \lif (R \wedge S) \sststile{}{} (R \wedge S) \lif (R \vee S)}
  }
  [\vver{v} (R \vee S) \lif T, name=prem1,just=Premisa
    [\vver{v} T \lif (R \wedge S), name=prem2,just=Premisa
      [\vver{f} (R \wedge S) \lif (R \vee S), name=conc,just=Conclusión
        [\vver{v} R \wedge S, just=FI:conc
          [\vver{f} R \vee S, just=FI:conc
            [\vver{f} R \vee S, just=VI:prem1]
            [\vver{v} T, just=VI:prem1, name=viprem1
              [\vver{f} T, just=VI:prem2, close={:viprem1,!c}]
              [\vver{v} R \wedge S, just=VI:prem2]
            ]
          ]
        ]
      ]
    ]
  ]
\end{prooftree}

% \item
\begin{prooftree}
  {
    to prove={U \lif (V \vee W), (V \wedge W) \lif \lnot U \sststile{}{} \lnot U}
  }
  [\vver{v} U \lif (V \vee W), name=prem1,just=Premisa
    [\vver{v} (V \wedge W) \lif \lnot U, name=prem2, just=Premisa
      [\vver{f} \lnot U, name=conc,just=Conclusión
        [\vver{f} V \wedge W, just=VI:prem2
          [\vver{f} U, just=VI:prem1, close={:conc,!c}]
          [\vver{v} V \vee W, just=VI:prem1]
        ]
        [\vver{v} \lnot U, close={:conc,!c}]
      ]
    ]
  ]
\end{prooftree}


\end{document}
