%\documentclass[border=10pt,tikz,letter]{standalone}
\documentclass[10pt,british,letter]{ltxdoc}
\usepackage{prooftrees,turnstile}
\newcommand*{\lif}{\ensuremath{\mathbin{\rightarrow}}}

\newcommand\vver[1]{\textcolor{red}{\textit{#1 }}}

\begin{document}

Pruebe la invalidez de los siguientes argumentos.

% \begin{prooftree}
% {
% to prove={\{P \vee (Q \vee \lnot R), P \lif \lnot R, Q \lif \lnot R\} \sststile{}{} \lnot R}
% }
% [P \vee (Q \vee \lnot R),  just=Ass, checked
% [P \lif \lnot R,  just=Ass, checked
%   [Q \lif \lnot R,  just=Ass, checked, name=last premise
%     [\lnot\lnot R, just={$\lnot$ Conc}, name=not conc
%       [P,  just={$\vee$ Elim:!uuuu}
%         [\lnot P, close={:!u,!c}]
%         [\lnot R,  close={:not conc,!c}, just={$\lif$ Elim:!uuuu}]]
%       [Q \vee \lnot R
%         [Q, move by=1
%           [\lnot Q, close={:!u,!c}]
%           [\lnot R,  close={:not conc,!c}, just={$\lif$ Elim:last premise}]]
%         [\lnot R, close={:not conc,!c}, move by=1, just={$\vee$ Elim:!u}]]]]]]
% \end{prooftree}

1
\begin{prooftree}
{
  to prove={(\exists x) Ax \wedge Bx, (\exists x) Cx \wedge Bx \sststile{}{} (\forall x) Cx \lif \lnot Ax}
}
[\vver{v} (\exists x) Ax \wedge Bx, name=prem1
  [\vver{v} (\exists x) Cx \wedge Bx, name=prem2
    [\vver{f} (\forall x) Cx \lif \lnot Ax, name=conc
      [\vver{v} Aa \wedge Ba, just=VP:prem1, name=vpprem1
        [\vver{v} Cb \wedge Bb, just=VP:prem2, name=vpprem2
          [\vver{f} Cc \lif \lnot Ac, just=FG:conc, name=fgconc
            [\vver{v} Aa, just=VC:vpprem1
              [\vver{v} Ba, just=VC:vpprem1
                [\vver{v} Cb, just=VC:vpprem2
                  [\vver{v} Bb, just=VC:vpprem2
                    [\vver{v} Cc, just=FI:fgconc
                      [\vver{f} \lnot Ac, just=FI:fgconc]
                    ]
                  ]
                ]
              ]
            ]
          ]
        ]
      ]
    ]
  ]
]
\end{prooftree}

2
\begin{prooftree}
{
  to prove={(\forall x) Dx \lif \lnot Ex, (\forall x) Ex \lif Fx \sststile{}{} (\forall x) Fx \lif \lnot Dx}
}
[\vver{v} (\forall x) Dx \lif \lnot Ex, name=prem1
  [\vver{v} (\forall x) Ex \lif Fx, name=prem2
    [\vver{f} (\forall x) Fx \lif \lnot Dx, name=conc
      [\vver{v} Da \lif \lnot Ea, just=VG:prem1, name=vpprem1
        [\vver{v} Ea \lif Fa, just=VG:prem2, name=vpprem2
          [\vver{f} Fa \lif \lnot Da, just=FG:conc, name=fgconc
            [\vver{v} Fa, just=FI:fgconc, name=fifgconcant
              [\vver{f} \lnot Da, just=FI:fgconc, name=fifgconccon
                [\vver{f} Da, just=VI:vpprem1, close={:fifgconccon,!c}]
                [\vver{v} \lnot Ea, just=VI:vpprem1
                    [\vver{f} Ea, just=VI:VI:vpprem2]
                    [\vver{v} Fa, just=VI:vpprem2]
                ]
              ]
            ]
          ]
        ]
      ]
    ]
  ]
]
\end{prooftree}
\newline
I=$\langle U, D^{*},E^{*},F^{*} \rangle$ \newline
U=\{a\} \newline
$D^{*}$=\{a\} \newline
$E^{*}$=\{a\} \newline
$F^{*}$=\{a\} \newline

3
\begin{prooftree}
{
  to prove={(\forall x) Gx \lif Hx, (\forall x) Gx \lif Ix \sststile{}{} (\forall x) Ix \lif Hx}
}
[\vver{v} (\forall x) Gx \lif Hx, name=prem1
  [\vver{v} (\forall x) Gx \lif Ix, name=prem2
    [\vver{f} (\forall x) Ix \lif Hx, name=conc
      [\vver{f} Ia \lif Ha, just=FG:conc, name=fgConc
        [\vver{v} Ia, just=FI:fgConc, name=fiConcAnt
          [\vver{f} Ha, just=FI:fgConc, name=fiConcCons
            [\vver{v} Ga \lif Ha, just=VG:prem1
              [\vver{f} Ga
                [\vver{v} Ga \lif Ia
                  [\vver{f} Ga]
                  [\vver{v} Ia]
                ]
              ]
              [\vver{v} Ha, close={:fiConcCons,!c}]
            ]
          ]
        ]
      ]
    ]
  ]
]
\end{prooftree}
\newline
I=$\langle U, G^{*},H^{*},I^{*} \rangle$ \newline
U=\{a\} \newline
$G^{*}$=\{$\emptyset$\} \newline
$H^{*}$=\{$\emptyset$\} \newline
$I^{*}$=\{a\} \newline

4
\begin{prooftree}
{
  to prove={(\exists x) Jx \wedge Kx, (\exists x) Kx \wedge Lx \sststile{}{} (\exists x) Lx \wedge Jx}
}
[\vver{v} (\exists x) Jx \wedge Kx, name=prem1
  [\vver{v} (\exists x) Kx \wedge Lx, name=prem2
    [\vver{f} (\exists x) Lx \wedge Jx, name=conc
      [\vver{v} Ja \wedge Ka, just=VP:prem1, name=vpPrem1
        [\vver{v} Ja, just=VC:vpPrem1
          [\vver{v} Ka, just=VC:vpPrem1
            [\vver{v} Kb \wedge Lb, just=VP:prem2, name=vpPrem2
              [\vver{v} Kb, just=VC:vpPrem2
                [\vver{v} Lb, just=VC:vpPrem2, name=vcPrem2Cons
                  [\vver{f} Lb \wedge Jb, just=FP:conc, name=fpConc
                    [\vver{f} Lb, just=FC:fpConc, close={:vcPrem2Cons,!c}]
                    [\vver{f} Jb, just=FC:fpConc]
                  ]
                ]
              ]
            ]
          ]
        ]
      ]
    ]
  ]
]
\end{prooftree}
\newline
I=$\langle U, G^{*},H^{*},I^{*} \rangle$ \newline
U=\{a\} \newline
$G^{*}=\{\emptyset\}$ \newline
$H^{*}=\{\emptyset\}$ \newline
$I^{*}=\{a\}$ \newline

5
\begin{prooftree}
{
  to prove={(\exists x) Mx \wedge Nx, (\exists x) Mx \wedge Ox \sststile{}{} (\forall x) Ox \lif Nx}
}
[\vver{v} (\exists x) Mx \wedge Nx, name=prem1
  [\vver{v} (\exists x) Mx \wedge Ox, name=prem2
    [\vver{f} (\forall x) Ox \lif Nx, name=conc
      [\vver{f} Oa \lif Na, just=FG:conc, name=fgConc
        [\vver{v} Oa, just=FI:fgConc
          [\vver{f} Na, just=FI:fgConc
            [\vver{v} Mb \wedge Nb, just=VP:prem1, name=vpPrem1
              [\vver{v} Mb, just=VC:vpPrem1
                [\vver{v} Nb, just=VC:vpPrem1, name=vcPrem1Cons
                  [\vver{v} Mc \wedge Oc, just=VP:prem2, name=vpPrem2
                    [\vver{v} Mc, just=VC:vpPrem2
                      [\vver{v} Oc, just=VC:vpPrem2]
                    ]
                  ]
                ]
              ]
            ]
          ]
        ]
      ]
    ]
  ]
]
\end{prooftree}
\newline
I=$\langle U, M^{*},N^{*},O^{*} \rangle$ \newline
U=\{a, b, c\} \newline
$M^{*}=\{c, b\}$ \newline
$N^{*}=\{b\}$ \newline
$O^{*}=\{c, a\}$ \newline

\end{document}
